\documentclass{standalone}
\usepackage{tikz,lmodern,amssymb}
\usepackage{knowledge}

\begin{document}

\begin{defn*}
{A Formula's Variable Replaced by a Term}
Suppose that \(\phi\) is an \(\mathcal{L}\)-formula, \(t\) is a term, and \(x\) is a variable. We define the formula \(\phi_{t}^{x}\) (read ``\(\phi\) with \(x\) replaced by $ t $") as follows:
\begin{enumerate}
    \item If \(\phi: \equiv = u_{1} u_{2}\), then \(\phi_{t}^{x}\) is \( = \left(u_{1}\right)_{t}^{x}\left(u_{2}\right)_{t}^{x}\). 
    \item If \(\phi: \equiv R u_{1} u_{2} \ldots u_{n}\), then \(\phi_{t}^{x}\) is \(R\left(u_{1}\right)_{t}^{x}\left(u_{2}\right)_{t}^{x} \ldots\left(u_{n}\right)_{t}^{x}\)
    \item If \(\phi: \equiv \neg(\alpha)\), then \(\phi_{t}^{x}\) is \(\neg\left(\alpha_{t}^{x}\right)\).
    \item If \(\phi: \equiv(\alpha \vee \beta)\), then \(\phi_{t}^{x}\) is \(\left(\alpha_{t}^{x} \vee \beta_{t}^{x}\right)\)
    \item If \(\phi: \equiv(\forall y)(\alpha)\), then
    \[
    \phi_{t}^{x} =
\begin{cases}
\phi & \text { if } x \text { is } y \\
 (\forall y)\left(\alpha_{t}^{x}\right) & \text {otherwise}
\end{cases}
    \]
\end{enumerate}

\begin{ex}
Suppose that \(\phi\) is the formula
\[
P(x, y) \rightarrow[(\forall x)(Q(g(x), z)) \vee(\forall y)(R(x, h(x))]
\]
Then, if \(t\) is the term \(g(c)\), we get
\[
\phi_{t}^{x} \text { is } P(g(c), y) \rightarrow[(\forall x)(Q(g(x), z)) \vee(\forall y)(R(g(c), h(g(c)))]
\]
\end{ex}

\end{defn*}

\end{document}
