\begin{definition}{Conditional Independence}{conditional_independence}
Suppose $ A $ and $ B $ are independent events, then we would want $ P\left( A \mid C  \right) =  P\left( A \mid B \cap C  \right)  $:
\[
P\left( A \mid C \right) = \frac{P\left( A \cap C \right) }{P\left( C \right) } ~\text{and}~  P\left( A \mid B \cap  C \right) =  \frac{P\left( A \cap  B \cap  C \right) }{P\left( B \cap  C \right) }
\]
So then we want:
\begin{gather*}
    P\left( A \mid C \right) =  P\left( A \mid B \cap  C \right)  \\
    \Updownarrow \\
\frac{P\left( A \cap C \right) }{P\left( C \right) } =  \frac{P\left( A \cap  B \cap  C \right) }{P\left( B \cap  C \right) }\\
    \Updownarrow \\
    \frac{P\left( A \cap B \cap  C \right) }{P\left( C \right) } =  \frac{P\left( A \cap  C \right) P\left( B \cap  C \right)  }{ P\left( C \right) P\left( C \right)  }\\
    \Updownarrow \\
    P\left( A \cap B \mid C \right)  =  P\left( A \mid C \right) P\left( B \mid C \right) 
\end{gather*}
\end{definition}
